make unverified.c compile
I used the sel4 docker file and follow the instructions to set up sel4test for odroid-c2 platform.
Then, using ninja -v, I could list the required include paths.

verified_cogent_driver/unverified.c
@@ -1,17 +1,11 @@
+#include "meson_timer.h"
 
-#define TIMER_BASE      0xc1100000
-#define TIMER_MAP_BASE  0xc1109000
-
-#define TIMER_REG_START   0x2650    // TIMER_MUX
-
-typedef unsigned int    uint32_t;
-typedef uint32_t uintptr_t;
-
-typedef struct {
-    void *vaddr;
-} meson_timer_config_t;
-
-#include "generated/driver.cogent"
+#include <errno.h>
+#include <stdlib.h>
+#include <utils/util.h>
+#include <platsupport/timer.h>
+#include <platsupport/plat/meson_timer.h>
+#include "generated/driver.c"
 
 /*
 
@@ -28,7 +22,16 @@ int meson_init(meson_timer_t *timer, meson_timer_config_t config)
     }
 
     timer->regs = (void *)((uintptr_t) config.vaddr + (TIMER_BASE + TIMER_REG_START * 4 - TIMER_MAP_BASE));
-    initialize(timer);
+    meson_init_cogent((Meson_timer *) timer);
     return 0;
 }
-   
+
+uint64_t meson_get_time(meson_timer_t *timer) {
+    return meson_get_time_cogent((Meson_timer *) timer);
+}
+void meson_set_timeout(meson_timer_t *timer, uint16_t timeout, bool periodic) {
+    meson_set_timeout_cogent ((TimeoutInput) { (Meson_timer *) timer, timeout, periodic });
+}
+void meson_stop_timer(meson_timer_t *timer) {
+    meson_stop_timer_cogent((Meson_timer*) timer);
+}
