verified_cogent_driver/generated/Driver_ShallowTuplesProof.thy
@@ -29,31 +29,31 @@ structure ShallowTuplesThms_Driver =
 setup \<open> ShallowTuplesThms_Driver.setup \<close>
 
 
-overloading shallow_tuples_rel_T0 \<equiv> shallow_tuples_rel begin
-  definition "shallow_tuples_rel_T0 (x :: ('x1, 'x2, 'x3) Driver_ShallowShared.T0) (xt :: 'xt1 \<times> 'xt2 \<times> 'xt3) \<equiv>
-    shallow_tuples_rel (Driver_ShallowShared.T0.p1\<^sub>f x) (prod.fst xt) \<and>
-    shallow_tuples_rel (Driver_ShallowShared.T0.p2\<^sub>f x) (prod.fst (prod.snd xt)) \<and>
-    shallow_tuples_rel (Driver_ShallowShared.T0.p3\<^sub>f x) (prod.snd (prod.snd xt))"
+overloading shallow_tuples_rel_TimeoutInput \<equiv> shallow_tuples_rel begin
+  definition "shallow_tuples_rel_TimeoutInput (x :: ('x1, 'x2, 'x3) Driver_ShallowShared.TimeoutInput) (xt :: 'xt1 \<times> 'xt2 \<times> 'xt3) \<equiv>
+    shallow_tuples_rel (Driver_ShallowShared.TimeoutInput.p1\<^sub>f x) (prod.fst xt) \<and>
+    shallow_tuples_rel (Driver_ShallowShared.TimeoutInput.p2\<^sub>f x) (prod.fst (prod.snd xt)) \<and>
+    shallow_tuples_rel (Driver_ShallowShared.TimeoutInput.p3\<^sub>f x) (prod.snd (prod.snd xt))"
 end
-lemma shallow_tuples_rule__T0_make [ShallowTuplesRules_Driver]:
+lemma shallow_tuples_rule__TimeoutInput_make [ShallowTuplesRules_Driver]:
   "\<lbrakk>
      shallow_tuples_rel x1 xt1;
      shallow_tuples_rel x2 xt2;
      shallow_tuples_rel x3 xt3
-  \<rbrakk> \<Longrightarrow> shallow_tuples_rel (Driver_ShallowShared.T0.make x1 x2 x3) (xt1, xt2, xt3)"
-  by (simp add: shallow_tuples_rel_T0_def Driver_ShallowShared.T0.defs Px_px)
-lemma shallow_tuples_rule__T0__p1\<^sub>f [ShallowTuplesThms_Driver]:
-  "shallow_tuples_rel (x :: ('x1, 'x2, 'x3) Driver_ShallowShared.T0) (xt :: 'xt1 \<times> 'xt2 \<times> 'xt3) \<Longrightarrow>
-   shallow_tuples_rel (Driver_ShallowShared.T0.p1\<^sub>f x) (prod.fst xt)"
-  by (simp add: shallow_tuples_rel_T0_def)
-lemma shallow_tuples_rule__T0__p2\<^sub>f [ShallowTuplesThms_Driver]:
-  "shallow_tuples_rel (x :: ('x1, 'x2, 'x3) Driver_ShallowShared.T0) (xt :: 'xt1 \<times> 'xt2 \<times> 'xt3) \<Longrightarrow>
-   shallow_tuples_rel (Driver_ShallowShared.T0.p2\<^sub>f x) (prod.fst (prod.snd xt))"
-  by (simp add: shallow_tuples_rel_T0_def)
-lemma shallow_tuples_rule__T0__p3\<^sub>f [ShallowTuplesThms_Driver]:
-  "shallow_tuples_rel (x :: ('x1, 'x2, 'x3) Driver_ShallowShared.T0) (xt :: 'xt1 \<times> 'xt2 \<times> 'xt3) \<Longrightarrow>
-   shallow_tuples_rel (Driver_ShallowShared.T0.p3\<^sub>f x) (prod.snd (prod.snd xt))"
-  by (simp add: shallow_tuples_rel_T0_def)
+  \<rbrakk> \<Longrightarrow> shallow_tuples_rel (Driver_ShallowShared.TimeoutInput.make x1 x2 x3) (xt1, xt2, xt3)"
+  by (simp add: shallow_tuples_rel_TimeoutInput_def Driver_ShallowShared.TimeoutInput.defs Px_px)
+lemma shallow_tuples_rule__TimeoutInput__p1\<^sub>f [ShallowTuplesThms_Driver]:
+  "shallow_tuples_rel (x :: ('x1, 'x2, 'x3) Driver_ShallowShared.TimeoutInput) (xt :: 'xt1 \<times> 'xt2 \<times> 'xt3) \<Longrightarrow>
+   shallow_tuples_rel (Driver_ShallowShared.TimeoutInput.p1\<^sub>f x) (prod.fst xt)"
+  by (simp add: shallow_tuples_rel_TimeoutInput_def)
+lemma shallow_tuples_rule__TimeoutInput__p2\<^sub>f [ShallowTuplesThms_Driver]:
+  "shallow_tuples_rel (x :: ('x1, 'x2, 'x3) Driver_ShallowShared.TimeoutInput) (xt :: 'xt1 \<times> 'xt2 \<times> 'xt3) \<Longrightarrow>
+   shallow_tuples_rel (Driver_ShallowShared.TimeoutInput.p2\<^sub>f x) (prod.fst (prod.snd xt))"
+  by (simp add: shallow_tuples_rel_TimeoutInput_def)
+lemma shallow_tuples_rule__TimeoutInput__p3\<^sub>f [ShallowTuplesThms_Driver]:
+  "shallow_tuples_rel (x :: ('x1, 'x2, 'x3) Driver_ShallowShared.TimeoutInput) (xt :: 'xt1 \<times> 'xt2 \<times> 'xt3) \<Longrightarrow>
+   shallow_tuples_rel (Driver_ShallowShared.TimeoutInput.p3\<^sub>f x) (prod.snd (prod.snd xt))"
+  by (simp add: shallow_tuples_rel_TimeoutInput_def)
 
 
 overloading shallow_tuples_rel_Meson_timer \<equiv> shallow_tuples_rel begin
@@ -184,10 +184,10 @@ lemma shallow_tuples_rule__Meson_timer_reg__timer_e_input_clk\<^sub>f__update [S
 
 overloading shallow_tuples_rel_Timeout_timebase \<equiv> shallow_tuples_rel begin
   definition "shallow_tuples_rel_Timeout_timebase (x :: ('x1, 'x2, 'x3, 'x4) Driver_ShallowShared.Timeout_timebase) (xt :: ('xt1, 'xt2, 'xt3, 'xt4) Driver_ShallowShared_Tuples.Timeout_timebase) \<equiv>
-    (\<exists>v vt. shallow_tuples_rel v vt \<and> x = Driver_ShallowShared.Timeout_timebase.TIMEOUT_TIMEBASE_100_US v \<and> xt = Driver_ShallowShared_Tuples.Timeout_timebase.TIMEOUT_TIMEBASE_100_US vt) \<or>
-    (\<exists>v vt. shallow_tuples_rel v vt \<and> x = Driver_ShallowShared.Timeout_timebase.TIMEOUT_TIMEBASE_10_US v \<and> xt = Driver_ShallowShared_Tuples.Timeout_timebase.TIMEOUT_TIMEBASE_10_US vt) \<or>
-    (\<exists>v vt. shallow_tuples_rel v vt \<and> x = Driver_ShallowShared.Timeout_timebase.TIMEOUT_TIMEBASE_1_MS v \<and> xt = Driver_ShallowShared_Tuples.Timeout_timebase.TIMEOUT_TIMEBASE_1_MS vt) \<or>
-    (\<exists>v vt. shallow_tuples_rel v vt \<and> x = Driver_ShallowShared.Timeout_timebase.TIMEOUT_TIMEBASE_1_US v \<and> xt = Driver_ShallowShared_Tuples.Timeout_timebase.TIMEOUT_TIMEBASE_1_US vt)"
+    (\<exists>v vt. shallow_tuples_rel v vt \<and> x = Driver_ShallowShared.Timeout_timebase.COGENT_TIMEOUT_TIMEBASE_100_US v \<and> xt = Driver_ShallowShared_Tuples.Timeout_timebase.COGENT_TIMEOUT_TIMEBASE_100_US vt) \<or>
+    (\<exists>v vt. shallow_tuples_rel v vt \<and> x = Driver_ShallowShared.Timeout_timebase.COGENT_TIMEOUT_TIMEBASE_10_US v \<and> xt = Driver_ShallowShared_Tuples.Timeout_timebase.COGENT_TIMEOUT_TIMEBASE_10_US vt) \<or>
+    (\<exists>v vt. shallow_tuples_rel v vt \<and> x = Driver_ShallowShared.Timeout_timebase.COGENT_TIMEOUT_TIMEBASE_1_MS v \<and> xt = Driver_ShallowShared_Tuples.Timeout_timebase.COGENT_TIMEOUT_TIMEBASE_1_MS vt) \<or>
+    (\<exists>v vt. shallow_tuples_rel v vt \<and> x = Driver_ShallowShared.Timeout_timebase.COGENT_TIMEOUT_TIMEBASE_1_US v \<and> xt = Driver_ShallowShared_Tuples.Timeout_timebase.COGENT_TIMEOUT_TIMEBASE_1_US vt)"
 end
 lemma shallow_tuples_rule_case__Timeout_timebase [ShallowTuplesThms_Driver]:
   "\<lbrakk> shallow_tuples_rel x xt;
@@ -199,31 +199,31 @@ lemma shallow_tuples_rule_case__Timeout_timebase [ShallowTuplesThms_Driver]:
    shallow_tuples_rel (Driver_ShallowShared.case_Timeout_timebase f1 f2 f3 f4 x) (Driver_ShallowShared_Tuples.case_Timeout_timebase ft1 ft2 ft3 ft4 xt)"
   by (fastforce simp: shallow_tuples_rel_Timeout_timebase_def
         split: Driver_ShallowShared.Timeout_timebase.splits Driver_ShallowShared_Tuples.Timeout_timebase.splits)
-lemma shallow_tuples_rule__Timeout_timebase__TIMEOUT_TIMEBASE_100_US [ShallowTuplesRules_Driver]:
+lemma shallow_tuples_rule__Timeout_timebase__COGENT_TIMEOUT_TIMEBASE_100_US [ShallowTuplesRules_Driver]:
   "shallow_tuples_rel x xt \<Longrightarrow>
-   shallow_tuples_rel (Driver_ShallowShared.Timeout_timebase.TIMEOUT_TIMEBASE_100_US x) (Driver_ShallowShared_Tuples.Timeout_timebase.TIMEOUT_TIMEBASE_100_US xt)"
+   shallow_tuples_rel (Driver_ShallowShared.Timeout_timebase.COGENT_TIMEOUT_TIMEBASE_100_US x) (Driver_ShallowShared_Tuples.Timeout_timebase.COGENT_TIMEOUT_TIMEBASE_100_US xt)"
   by (simp add: shallow_tuples_rel_Timeout_timebase_def)
-lemma shallow_tuples_rule__Timeout_timebase__TIMEOUT_TIMEBASE_10_US [ShallowTuplesRules_Driver]:
+lemma shallow_tuples_rule__Timeout_timebase__COGENT_TIMEOUT_TIMEBASE_10_US [ShallowTuplesRules_Driver]:
   "shallow_tuples_rel x xt \<Longrightarrow>
-   shallow_tuples_rel (Driver_ShallowShared.Timeout_timebase.TIMEOUT_TIMEBASE_10_US x) (Driver_ShallowShared_Tuples.Timeout_timebase.TIMEOUT_TIMEBASE_10_US xt)"
+   shallow_tuples_rel (Driver_ShallowShared.Timeout_timebase.COGENT_TIMEOUT_TIMEBASE_10_US x) (Driver_ShallowShared_Tuples.Timeout_timebase.COGENT_TIMEOUT_TIMEBASE_10_US xt)"
   by (simp add: shallow_tuples_rel_Timeout_timebase_def)
-lemma shallow_tuples_rule__Timeout_timebase__TIMEOUT_TIMEBASE_1_MS [ShallowTuplesRules_Driver]:
+lemma shallow_tuples_rule__Timeout_timebase__COGENT_TIMEOUT_TIMEBASE_1_MS [ShallowTuplesRules_Driver]:
   "shallow_tuples_rel x xt \<Longrightarrow>
-   shallow_tuples_rel (Driver_ShallowShared.Timeout_timebase.TIMEOUT_TIMEBASE_1_MS x) (Driver_ShallowShared_Tuples.Timeout_timebase.TIMEOUT_TIMEBASE_1_MS xt)"
+   shallow_tuples_rel (Driver_ShallowShared.Timeout_timebase.COGENT_TIMEOUT_TIMEBASE_1_MS x) (Driver_ShallowShared_Tuples.Timeout_timebase.COGENT_TIMEOUT_TIMEBASE_1_MS xt)"
   by (simp add: shallow_tuples_rel_Timeout_timebase_def)
-lemma shallow_tuples_rule__Timeout_timebase__TIMEOUT_TIMEBASE_1_US [ShallowTuplesRules_Driver]:
+lemma shallow_tuples_rule__Timeout_timebase__COGENT_TIMEOUT_TIMEBASE_1_US [ShallowTuplesRules_Driver]:
   "shallow_tuples_rel x xt \<Longrightarrow>
-   shallow_tuples_rel (Driver_ShallowShared.Timeout_timebase.TIMEOUT_TIMEBASE_1_US x) (Driver_ShallowShared_Tuples.Timeout_timebase.TIMEOUT_TIMEBASE_1_US xt)"
+   shallow_tuples_rel (Driver_ShallowShared.Timeout_timebase.COGENT_TIMEOUT_TIMEBASE_1_US x) (Driver_ShallowShared_Tuples.Timeout_timebase.COGENT_TIMEOUT_TIMEBASE_1_US xt)"
   by (simp add: shallow_tuples_rel_Timeout_timebase_def)
 
 
 overloading shallow_tuples_rel_Timestamp_timebase \<equiv> shallow_tuples_rel begin
   definition "shallow_tuples_rel_Timestamp_timebase (x :: ('x1, 'x2, 'x3, 'x4, 'x5) Driver_ShallowShared.Timestamp_timebase) (xt :: ('xt1, 'xt2, 'xt3, 'xt4, 'xt5) Driver_ShallowShared_Tuples.Timestamp_timebase) \<equiv>
-    (\<exists>v vt. shallow_tuples_rel v vt \<and> x = Driver_ShallowShared.Timestamp_timebase.TIMESTAMP_TIMEBASE_100_US v \<and> xt = Driver_ShallowShared_Tuples.Timestamp_timebase.TIMESTAMP_TIMEBASE_100_US vt) \<or>
-    (\<exists>v vt. shallow_tuples_rel v vt \<and> x = Driver_ShallowShared.Timestamp_timebase.TIMESTAMP_TIMEBASE_10_US v \<and> xt = Driver_ShallowShared_Tuples.Timestamp_timebase.TIMESTAMP_TIMEBASE_10_US vt) \<or>
-    (\<exists>v vt. shallow_tuples_rel v vt \<and> x = Driver_ShallowShared.Timestamp_timebase.TIMESTAMP_TIMEBASE_1_MS v \<and> xt = Driver_ShallowShared_Tuples.Timestamp_timebase.TIMESTAMP_TIMEBASE_1_MS vt) \<or>
-    (\<exists>v vt. shallow_tuples_rel v vt \<and> x = Driver_ShallowShared.Timestamp_timebase.TIMESTAMP_TIMEBASE_1_US v \<and> xt = Driver_ShallowShared_Tuples.Timestamp_timebase.TIMESTAMP_TIMEBASE_1_US vt) \<or>
-    (\<exists>v vt. shallow_tuples_rel v vt \<and> x = Driver_ShallowShared.Timestamp_timebase.TIMESTAMP_TIMEBASE_SYSTEM v \<and> xt = Driver_ShallowShared_Tuples.Timestamp_timebase.TIMESTAMP_TIMEBASE_SYSTEM vt)"
+    (\<exists>v vt. shallow_tuples_rel v vt \<and> x = Driver_ShallowShared.Timestamp_timebase.COGENT_TIMESTAMP_TIMEBASE_100_US v \<and> xt = Driver_ShallowShared_Tuples.Timestamp_timebase.COGENT_TIMESTAMP_TIMEBASE_100_US vt) \<or>
+    (\<exists>v vt. shallow_tuples_rel v vt \<and> x = Driver_ShallowShared.Timestamp_timebase.COGENT_TIMESTAMP_TIMEBASE_10_US v \<and> xt = Driver_ShallowShared_Tuples.Timestamp_timebase.COGENT_TIMESTAMP_TIMEBASE_10_US vt) \<or>
+    (\<exists>v vt. shallow_tuples_rel v vt \<and> x = Driver_ShallowShared.Timestamp_timebase.COGENT_TIMESTAMP_TIMEBASE_1_MS v \<and> xt = Driver_ShallowShared_Tuples.Timestamp_timebase.COGENT_TIMESTAMP_TIMEBASE_1_MS vt) \<or>
+    (\<exists>v vt. shallow_tuples_rel v vt \<and> x = Driver_ShallowShared.Timestamp_timebase.COGENT_TIMESTAMP_TIMEBASE_1_US v \<and> xt = Driver_ShallowShared_Tuples.Timestamp_timebase.COGENT_TIMESTAMP_TIMEBASE_1_US vt) \<or>
+    (\<exists>v vt. shallow_tuples_rel v vt \<and> x = Driver_ShallowShared.Timestamp_timebase.COGENT_TIMESTAMP_TIMEBASE_SYSTEM v \<and> xt = Driver_ShallowShared_Tuples.Timestamp_timebase.COGENT_TIMESTAMP_TIMEBASE_SYSTEM vt)"
 end
 lemma shallow_tuples_rule_case__Timestamp_timebase [ShallowTuplesThms_Driver]:
   "\<lbrakk> shallow_tuples_rel x xt;
@@ -236,25 +236,25 @@ lemma shallow_tuples_rule_case__Timestamp_timebase [ShallowTuplesThms_Driver]:
    shallow_tuples_rel (Driver_ShallowShared.case_Timestamp_timebase f1 f2 f3 f4 f5 x) (Driver_ShallowShared_Tuples.case_Timestamp_timebase ft1 ft2 ft3 ft4 ft5 xt)"
   by (fastforce simp: shallow_tuples_rel_Timestamp_timebase_def
         split: Driver_ShallowShared.Timestamp_timebase.splits Driver_ShallowShared_Tuples.Timestamp_timebase.splits)
-lemma shallow_tuples_rule__Timestamp_timebase__TIMESTAMP_TIMEBASE_100_US [ShallowTuplesRules_Driver]:
+lemma shallow_tuples_rule__Timestamp_timebase__COGENT_TIMESTAMP_TIMEBASE_100_US [ShallowTuplesRules_Driver]:
   "shallow_tuples_rel x xt \<Longrightarrow>
-   shallow_tuples_rel (Driver_ShallowShared.Timestamp_timebase.TIMESTAMP_TIMEBASE_100_US x) (Driver_ShallowShared_Tuples.Timestamp_timebase.TIMESTAMP_TIMEBASE_100_US xt)"
+   shallow_tuples_rel (Driver_ShallowShared.Timestamp_timebase.COGENT_TIMESTAMP_TIMEBASE_100_US x) (Driver_ShallowShared_Tuples.Timestamp_timebase.COGENT_TIMESTAMP_TIMEBASE_100_US xt)"
   by (simp add: shallow_tuples_rel_Timestamp_timebase_def)
-lemma shallow_tuples_rule__Timestamp_timebase__TIMESTAMP_TIMEBASE_10_US [ShallowTuplesRules_Driver]:
+lemma shallow_tuples_rule__Timestamp_timebase__COGENT_TIMESTAMP_TIMEBASE_10_US [ShallowTuplesRules_Driver]:
   "shallow_tuples_rel x xt \<Longrightarrow>
-   shallow_tuples_rel (Driver_ShallowShared.Timestamp_timebase.TIMESTAMP_TIMEBASE_10_US x) (Driver_ShallowShared_Tuples.Timestamp_timebase.TIMESTAMP_TIMEBASE_10_US xt)"
+   shallow_tuples_rel (Driver_ShallowShared.Timestamp_timebase.COGENT_TIMESTAMP_TIMEBASE_10_US x) (Driver_ShallowShared_Tuples.Timestamp_timebase.COGENT_TIMESTAMP_TIMEBASE_10_US xt)"
   by (simp add: shallow_tuples_rel_Timestamp_timebase_def)
-lemma shallow_tuples_rule__Timestamp_timebase__TIMESTAMP_TIMEBASE_1_MS [ShallowTuplesRules_Driver]:
+lemma shallow_tuples_rule__Timestamp_timebase__COGENT_TIMESTAMP_TIMEBASE_1_MS [ShallowTuplesRules_Driver]:
   "shallow_tuples_rel x xt \<Longrightarrow>
-   shallow_tuples_rel (Driver_ShallowShared.Timestamp_timebase.TIMESTAMP_TIMEBASE_1_MS x) (Driver_ShallowShared_Tuples.Timestamp_timebase.TIMESTAMP_TIMEBASE_1_MS xt)"
+   shallow_tuples_rel (Driver_ShallowShared.Timestamp_timebase.COGENT_TIMESTAMP_TIMEBASE_1_MS x) (Driver_ShallowShared_Tuples.Timestamp_timebase.COGENT_TIMESTAMP_TIMEBASE_1_MS xt)"
   by (simp add: shallow_tuples_rel_Timestamp_timebase_def)
-lemma shallow_tuples_rule__Timestamp_timebase__TIMESTAMP_TIMEBASE_1_US [ShallowTuplesRules_Driver]:
+lemma shallow_tuples_rule__Timestamp_timebase__COGENT_TIMESTAMP_TIMEBASE_1_US [ShallowTuplesRules_Driver]:
   "shallow_tuples_rel x xt \<Longrightarrow>
-   shallow_tuples_rel (Driver_ShallowShared.Timestamp_timebase.TIMESTAMP_TIMEBASE_1_US x) (Driver_ShallowShared_Tuples.Timestamp_timebase.TIMESTAMP_TIMEBASE_1_US xt)"
+   shallow_tuples_rel (Driver_ShallowShared.Timestamp_timebase.COGENT_TIMESTAMP_TIMEBASE_1_US x) (Driver_ShallowShared_Tuples.Timestamp_timebase.COGENT_TIMESTAMP_TIMEBASE_1_US xt)"
   by (simp add: shallow_tuples_rel_Timestamp_timebase_def)
-lemma shallow_tuples_rule__Timestamp_timebase__TIMESTAMP_TIMEBASE_SYSTEM [ShallowTuplesRules_Driver]:
+lemma shallow_tuples_rule__Timestamp_timebase__COGENT_TIMESTAMP_TIMEBASE_SYSTEM [ShallowTuplesRules_Driver]:
   "shallow_tuples_rel x xt \<Longrightarrow>
-   shallow_tuples_rel (Driver_ShallowShared.Timestamp_timebase.TIMESTAMP_TIMEBASE_SYSTEM x) (Driver_ShallowShared_Tuples.Timestamp_timebase.TIMESTAMP_TIMEBASE_SYSTEM xt)"
+   shallow_tuples_rel (Driver_ShallowShared.Timestamp_timebase.COGENT_TIMESTAMP_TIMEBASE_SYSTEM x) (Driver_ShallowShared_Tuples.Timestamp_timebase.COGENT_TIMESTAMP_TIMEBASE_SYSTEM xt)"
   by (simp add: shallow_tuples_rel_Timestamp_timebase_def)
 
 
@@ -268,40 +268,40 @@ lemma shallow_tuples__reset_timer_e [ShallowTuplesThms_Driver]:
            ShallowTuplesThms_Driver ShallowTuplesThms_Driver[THEN shallow_tuples_rel_funD])+
 
 
-lemma shallow_tuples__initialize [ShallowTuplesThms_Driver]:
-  "shallow_tuples_rel Driver_Shallow_Desugar.initialize Driver_Shallow_Desugar_Tuples.initialize"
+lemma shallow_tuples__meson_get_time_cogent [ShallowTuplesThms_Driver]:
+  "shallow_tuples_rel Driver_Shallow_Desugar.meson_get_time_cogent Driver_Shallow_Desugar_Tuples.meson_get_time_cogent"
   apply (rule shallow_tuples_rel_funI)
-  apply (unfold Driver_Shallow_Desugar.initialize_def Driver_Shallow_Desugar_Tuples.initialize_def id_def)
+  apply (unfold Driver_Shallow_Desugar.meson_get_time_cogent_def Driver_Shallow_Desugar_Tuples.meson_get_time_cogent_def id_def)
   apply ((unfold take\<^sub>c\<^sub>o\<^sub>g\<^sub>e\<^sub>n\<^sub>t_def Let\<^sub>d\<^sub>s_def Let_def split_def)?,(simp only: fst_conv snd_conv)?)
   by (assumption |
       rule shallow_tuples_basic_bucket ShallowTuplesRules_Driver
            ShallowTuplesThms_Driver ShallowTuplesThms_Driver[THEN shallow_tuples_rel_funD])+
 
 
-lemma shallow_tuples__meson_get_time [ShallowTuplesThms_Driver]:
-  "shallow_tuples_rel Driver_Shallow_Desugar.meson_get_time Driver_Shallow_Desugar_Tuples.meson_get_time"
+lemma shallow_tuples__meson_init_cogent [ShallowTuplesThms_Driver]:
+  "shallow_tuples_rel Driver_Shallow_Desugar.meson_init_cogent Driver_Shallow_Desugar_Tuples.meson_init_cogent"
   apply (rule shallow_tuples_rel_funI)
-  apply (unfold Driver_Shallow_Desugar.meson_get_time_def Driver_Shallow_Desugar_Tuples.meson_get_time_def id_def)
+  apply (unfold Driver_Shallow_Desugar.meson_init_cogent_def Driver_Shallow_Desugar_Tuples.meson_init_cogent_def id_def)
   apply ((unfold take\<^sub>c\<^sub>o\<^sub>g\<^sub>e\<^sub>n\<^sub>t_def Let\<^sub>d\<^sub>s_def Let_def split_def)?,(simp only: fst_conv snd_conv)?)
   by (assumption |
       rule shallow_tuples_basic_bucket ShallowTuplesRules_Driver
            ShallowTuplesThms_Driver ShallowTuplesThms_Driver[THEN shallow_tuples_rel_funD])+
 
 
-lemma shallow_tuples__meson_set_timeout [ShallowTuplesThms_Driver]:
-  "shallow_tuples_rel Driver_Shallow_Desugar.meson_set_timeout Driver_Shallow_Desugar_Tuples.meson_set_timeout"
+lemma shallow_tuples__meson_set_timeout_cogent [ShallowTuplesThms_Driver]:
+  "shallow_tuples_rel Driver_Shallow_Desugar.meson_set_timeout_cogent Driver_Shallow_Desugar_Tuples.meson_set_timeout_cogent"
   apply (rule shallow_tuples_rel_funI)
-  apply (unfold Driver_Shallow_Desugar.meson_set_timeout_def Driver_Shallow_Desugar_Tuples.meson_set_timeout_def id_def)
+  apply (unfold Driver_Shallow_Desugar.meson_set_timeout_cogent_def Driver_Shallow_Desugar_Tuples.meson_set_timeout_cogent_def id_def)
   apply ((unfold take\<^sub>c\<^sub>o\<^sub>g\<^sub>e\<^sub>n\<^sub>t_def Let\<^sub>d\<^sub>s_def Let_def split_def)?,(simp only: fst_conv snd_conv)?)
   by (assumption |
       rule shallow_tuples_basic_bucket ShallowTuplesRules_Driver
            ShallowTuplesThms_Driver ShallowTuplesThms_Driver[THEN shallow_tuples_rel_funD])+
 
 
-lemma shallow_tuples__meson_stop_timer [ShallowTuplesThms_Driver]:
-  "shallow_tuples_rel Driver_Shallow_Desugar.meson_stop_timer Driver_Shallow_Desugar_Tuples.meson_stop_timer"
+lemma shallow_tuples__meson_stop_timer_cogent [ShallowTuplesThms_Driver]:
+  "shallow_tuples_rel Driver_Shallow_Desugar.meson_stop_timer_cogent Driver_Shallow_Desugar_Tuples.meson_stop_timer_cogent"
   apply (rule shallow_tuples_rel_funI)
-  apply (unfold Driver_Shallow_Desugar.meson_stop_timer_def Driver_Shallow_Desugar_Tuples.meson_stop_timer_def id_def)
+  apply (unfold Driver_Shallow_Desugar.meson_stop_timer_cogent_def Driver_Shallow_Desugar_Tuples.meson_stop_timer_cogent_def id_def)
   apply ((unfold take\<^sub>c\<^sub>o\<^sub>g\<^sub>e\<^sub>n\<^sub>t_def Let\<^sub>d\<^sub>s_def Let_def split_def)?,(simp only: fst_conv snd_conv)?)
   by (assumption |
       rule shallow_tuples_basic_bucket ShallowTuplesRules_Driver
