verified_cogent_driver/generated/Driver_AllRefine.thy
@@ -83,9 +83,9 @@ fold (fn (f, thm) => Utils.define_lemmas (f ^ "_normalised") [thm] #> snd)
 locale Driver_cogent_shallow =
   "driver" + correspondence +
   constrains val_abs_typing :: "'b \<Rightarrow> name \<Rightarrow> type list \<Rightarrow> bool"
-         and upd_abs_typing :: "abstyp \<Rightarrow> name \<Rightarrow> type list \<Rightarrow> sigil \<Rightarrow> ptrtyp set \<Rightarrow> ptrtyp set \<Rightarrow> bool"
+         and upd_abs_typing :: "abstyp \<Rightarrow> name \<Rightarrow> type list \<Rightarrow> sigil \<Rightarrow> ptrtyp set \<Rightarrow> ptrtyp set \<Rightarrow> (funtyp, abstyp, ptrtyp) store \<Rightarrow> bool"
          and abs_repr       :: "abstyp \<Rightarrow> name \<times> repr list"
-         and abs_upd_val    :: "abstyp \<Rightarrow> 'b \<Rightarrow> char list \<Rightarrow> Cogent.type list \<Rightarrow> sigil \<Rightarrow> 32 word set \<Rightarrow> 32 word set \<Rightarrow> bool"
+         and abs_upd_val    :: "abstyp \<Rightarrow> 'b \<Rightarrow> char list \<Rightarrow> Cogent.type list \<Rightarrow> sigil \<Rightarrow> 32 word set \<Rightarrow> 32 word set \<Rightarrow> (char list, abstyp, 32 word) store \<Rightarrow> bool"
 
 
 sublocale Driver_cogent_shallow \<subseteq> Driver _ upd_abs_typing abs_repr
